L_Base: add execution

lean-formalisation/LeanFormalisation/LBase.lean
@@ -1,3 +1,4 @@
+import Mathlib.Data.Finmap
 import Mathlib.Tactic.Basic
 
 abbrev VarName := Nat
@@ -7,16 +8,23 @@ inductive τ
 | Bool
 deriving Repr
 
-inductive BinOp
-| Sub
-| Add
-| NatEq
-| BoolEq
-deriving Repr
 
-inductive UnOp
-| IsZero
-deriving Repr
+inductive Value
+| True
+| False
+| Nat (n : Nat)
+deriving Inhabited, Repr
+
+structure BinOp where
+  run : Value → Value → Value
+  arg1 : τ
+  arg2 : τ
+  out : τ
+
+structure UnOp where
+  run : Value → Value
+  arg : τ
+  out : τ
 
 inductive Expr
 | Var (x : VarName)
@@ -25,14 +33,15 @@ inductive Expr
 | Nat (n : Nat)
 | BinOp (arg₁ : Expr) (arg₂ : Expr) (op : BinOp)
 | UnOp (arg : Expr) (op : UnOp)
-deriving Repr
+
 
 inductive Stmt
 | Decl (x : VarName) (type : τ) (e : Expr)
 | Assign (x : VarName) (e : Expr)
 | Seq (s₁ : Stmt) (s₂ : Stmt)
 | If (e : Expr) (s₁ : Stmt) (s₂ : Stmt)
-deriving Repr
+| While (c : Expr) (body : Stmt)
+--| Break
 
 notation:100 s₁:100 ";" s₂:101 => Stmt.Seq s₁ s₂
 notation x "::=" exp => Stmt.Assign x exp
@@ -49,25 +58,13 @@ inductive ExprType : Γ → Expr → τ → Prop
 | VarAccess (x : VarName) (type : τ) :
   (Γ₁(x) = type) →
   ExprType Γ₁ (.Var x) type
-| IsZero (arg : Expr) :
-  ExprType Γ₁ arg .Nat →
-  ExprType Γ₁ (.UnOp arg .IsZero) .Bool
-| Sub (arg₁ arg₂ : Expr) :
-  ExprType Γ₁ arg₁ .Nat →
-  ExprType Γ₁ arg₂ .Nat →
-  ExprType Γ₁ (.BinOp arg₁ arg₂ .Sub) .Nat
-| Add (arg₁ arg₂ : Expr) :
-  ExprType Γ₁ arg₁ .Nat →
-  ExprType Γ₁ arg₂ .Nat →
-  ExprType Γ₁ (.BinOp arg₁ arg₂ .Add) .Nat
-| NatEq (arg₁ arg₂ : Expr) :
-  ExprType Γ₁ arg₁ .Nat →
-  ExprType Γ₁ arg₂ .Nat →
-  ExprType Γ₁ (.BinOp arg₁ arg₂ .NatEq) .Bool
-| BoolEq (arg₁ arg₂ : Expr) :
-  ExprType Γ₁ arg₁ .Bool →
-  ExprType Γ₁ arg₂ .Bool →
-  ExprType Γ₁ (.BinOp arg₁ arg₂ .BoolEq) .Bool
+| UnOp (arg : Expr) (type : τ) (out : τ) (run : Value → Value)  :
+  ExprType Γ₁ arg type →
+  ExprType Γ₁ (.UnOp arg ⟨run, type, out⟩) out
+| BinOp (arg₁ arg₂ : Expr) (type₁ : τ) (type₂ : τ) (out : τ) (run : Value → Value → Value) :
+  ExprType Γ₁ arg₁ type₁ →
+  ExprType Γ₁ arg₂ type₂ →
+  ExprType Γ₁ (.BinOp arg₁ arg₂ ⟨run, type₁, type₂, out⟩) out
 
 
 inductive StmtType : Γ → Stmt → Γ → Prop
@@ -79,10 +76,15 @@ inductive StmtType : Γ → Stmt → Γ → Prop
   StmtType Γ₁ (s₁; s₂) Γ₃
 | If (e : Expr) (s₁ s₂ : Stmt) : ExprType Γ₁ e .Bool → StmtType Γ₁ s₁ Γ₂ → StmtType Γ₁ s₂ Γ₃ →
   StmtType Γ₁ (.If e s₁ s₂) Γ₁
+| While (c : Expr) (s : Stmt) : ExprType Γ₁ c .Bool → StmtType Γ₁ s Γ₂ →
+  StmtType Γ₁ (.While c s) Γ₁
+/-| Break :
+  StmtType Γ₁ .Break Γ₂
+-/
 
 end Types
 
-section Properties
+section TypeProperties
 
 theorem StmtDet (Γ₁ Γ₂ Γ₃ : Γ) (s : Stmt) :
   StmtType Γ₁ s Γ₂ → StmtType Γ₁ s Γ₃ → Γ₂ = Γ₃ := by
@@ -113,8 +115,11 @@ lemma StmtMono (Γ₁ Γ₂ : Γ) (s : Stmt) :
       rcases s₂_ih Γ₂_1 Γ₂ a_1 with ⟨g2, hg2⟩
       exists g2 ++ g1
       grind }
+    { unhygienic cases hs
+      exists [] }
     unhygienic cases hs
     exists []
+
 
 lemma StmtDecl (type : τ) : StmtType Γ₁ (Stmt.Decl x type e) Γ₂ → Γ₂ = ⟨x, type⟩ :: Γ₁ := by
   grind [StmtType]
@@ -167,20 +172,37 @@ theorem StmtExtension (Γ₁ Γ₂ Γ₃ : Γ) (s : Stmt) :
         apply List.append_cancel_right
         apply hg1
       grind }
+    { by_cases hemp : Γ₂ = []
+      { simp only [hemp] at *
+        unhygienic cases hs
+        rcases StmtMono _ _ _ a_1 with ⟨g1, hg1⟩
+        rcases StmtMono _ _ _ a_2 with ⟨g2, hg2⟩
+        apply StmtType.If (Γ₂ := g1 ++ Γ₁ ++ Γ₃) (Γ₃ := g2 ++ Γ₁ ++ Γ₃)
+        { apply ExprExtension
+          apply a }
+        { apply s₁_ih
+          rw [hg1] at a_1
+          exact a_1 }
+        apply s₂_ih
+        rw [hg2] at a_2
+        exact a_2 }
+      have : Γ₂ ++ Γ₁ ≠ Γ₁ := by
+        intro eq
+        have : (Γ₂ ++ Γ₁).length > Γ₁.length := by
+          simp
+          grind
+        grind
+      grind [StmtType] }
     by_cases hemp : Γ₂ = []
     { simp only [hemp] at *
       unhygienic cases hs
       rcases StmtMono _ _ _ a_1 with ⟨g1, hg1⟩
-      rcases StmtMono _ _ _ a_2 with ⟨g2, hg2⟩
-      apply StmtType.If (Γ₂ := g1 ++ Γ₁ ++ Γ₃) (Γ₃ := g2 ++ Γ₁ ++ Γ₃)
+      apply StmtType.While (Γ₂ := g1 ++ Γ₁ ++ Γ₃)
       { apply ExprExtension
         apply a }
-      { apply s₁_ih
-        rw [hg1] at a_1
-        exact a_1 }
-      apply s₂_ih
-      rw [hg2] at a_2
-      exact a_2 }
+      apply body_ih
+      rw [hg1] at a_1
+      exact a_1 }
     have : Γ₂ ++ Γ₁ ≠ Γ₁ := by
       intro eq
       have : (Γ₂ ++ Γ₁).length > Γ₁.length := by
@@ -242,22 +264,40 @@ theorem StmtPermutation (Γ₁ Γ₂ Δ : Γ) (s : Stmt) :
           simp [List.find?_append] at *
           grind } }
       grind }
+    { by_cases hemp : Δ = []
+      { simp only [hemp] at *
+        unhygienic cases hs
+        rcases StmtMono _ _ _ a_1 with ⟨g1, hg1⟩
+        rcases StmtMono _ _ _ a_2 with ⟨g2, hg2⟩
+        apply StmtType.If (Γ₂ := g1 ++ Γ₂) (Γ₃ := g2 ++ Γ₂)
+        { apply ExprPermutation _ _ e .Bool heq
+          grind }
+        { apply s₁_ih Γ₁ Γ₂ g1
+          { grind }
+          rw [hg1] at a_1
+          exact a_1 }
+        apply s₂_ih Γ₁ Γ₂ g2
+        { grind }
+        rw [hg2] at a_2
+        exact a_2 }
+      have : Δ ++ Γ₁ ≠ Γ₁ := by
+        intro eq
+        have : (Δ ++ Γ₁).length > Γ₁.length := by
+          simp
+          grind
+        grind
+      grind [StmtType] }
     by_cases hemp : Δ = []
     { simp only [hemp] at *
       unhygienic cases hs
       rcases StmtMono _ _ _ a_1 with ⟨g1, hg1⟩
-      rcases StmtMono _ _ _ a_2 with ⟨g2, hg2⟩
-      apply StmtType.If (Γ₂ := g1 ++ Γ₂) (Γ₃ := g2 ++ Γ₂)
-      { apply ExprPermutation _ _ e .Bool heq
+      apply StmtType.While (Γ₂ := g1 ++ Γ₂)
+      { apply ExprPermutation _ _ c .Bool heq
         grind }
-      { apply s₁_ih Γ₁ Γ₂ g1
-        { grind }
-        rw [hg1] at a_1
-        exact a_1 }
-      apply s₂_ih Γ₁ Γ₂ g2
+      apply body_ih Γ₁ Γ₂ g1
       { grind }
-      rw [hg2] at a_2
-      exact a_2 }
+      rw [hg1] at a_1
+      exact a_1 }
     have : Δ ++ Γ₁ ≠ Γ₁ := by
       intro eq
       have : (Δ ++ Γ₁).length > Γ₁.length := by
@@ -266,4 +306,142 @@ theorem StmtPermutation (Γ₁ Γ₂ Δ : Γ) (s : Stmt) :
       grind
     grind [StmtType]
 
-end Properties
+end TypeProperties
+
+def liftValue : Value → Expr
+| .True => .True
+| .False => .False
+| .Nat (n : Nat) => .Nat n
+
+inductive Control
+| sourceExpr (e : Expr)
+| sourceStmt (s : Stmt)
+| value (v : Value)
+| skip
+
+abbrev Map (val : Type) := Finmap (fun _ : VarName ↦ val)
+
+abbrev Environment := List (Map Value)
+
+inductive Cont
+| ifCondK (s₁ s₂ : Stmt)
+| jumpK (l : Nat)
+| declK (x : VarName) (type : τ)
+| assignK (x : VarName)
+| seqK (s : Stmt)
+| binopLK (op : BinOp) (e₂ : Expr)
+| binopRK (op : BinOp) (v : Value)
+| unopK (op : UnOp)
+| loopK (c : Expr) (s : Stmt)
+
+abbrev CEK := Control × Environment × List Cont
+
+notation E "("x")!" => Option.get! (Finmap.lookup x (List.getD E 0 ∅ : Map Value) : Option Value)
+
+def popK (K : List Cont) (l : Nat) : List Cont :=
+  match K with
+  | .jumpK l₁ :: li => if l = l₁ then li else popK li l
+  | _ :: li => popK li l
+  | [] => panic! "popK from an empty List"
+
+def insert_first (key : VarName) (value : Value) : Environment → Environment
+| fst :: li => (Finmap.insert key value fst) :: li
+| [] => panic! "Insertion into empty environment"
+
+def modify_first (key : VarName) (value : Value) : Environment → Environment
+| fst :: li => (Finmap.insert key value (Finmap.erase key fst)) :: li
+| [] => panic! "Insertion into empty environment"
+
+
+inductive Eval : CEK → CEK → Prop
+-- # Expr
+| Val (v : Value) :
+  Eval
+    ⟨.sourceExpr (liftValue v), E, K⟩
+    ⟨.value v, E, K⟩
+| Var (v : Value) (x : VarName) :
+  Eval
+    ⟨.sourceExpr (.Var x), E, K⟩
+    ⟨.value (E(x)!), E, K⟩
+| If (e : Expr) (s₁ s₂ : Stmt) :
+  Eval
+    ⟨.sourceStmt (.If e s₁ s₂), E, K⟩
+    ⟨.sourceExpr e, E, (.ifCondK s₁ s₂) :: K⟩
+| VarDecl (x : VarName) (type : τ) (e : Expr) :
+  Eval
+    ⟨.sourceStmt (.Decl x type e), E, K⟩
+    ⟨.sourceExpr e, E, (.declK x type) :: K⟩
+| Assign (x : VarName) (e : Expr) :
+  Eval
+    ⟨.sourceStmt (.Assign x e), E, K⟩
+    ⟨.sourceExpr e, E, (.assignK x) :: K⟩
+| Seq (s₁ s₂ : Stmt) :
+  Eval
+    ⟨.sourceStmt (.Seq s₁ s₂), E, K⟩
+    ⟨.sourceStmt s₁, E, (.seqK s₂) :: K⟩
+| BinOp (e₁ e₂ : Expr) (op : BinOp) :
+  Eval
+    ⟨.sourceExpr (.BinOp e₁ e₂ op), E, K⟩
+    ⟨.sourceExpr e₁, E, (.binopLK op e₂) :: K⟩
+| UnOp (e : Expr) (op : UnOp) :
+  Eval
+    ⟨.sourceExpr (.UnOp e op), E, K⟩
+    ⟨.sourceExpr e, E, (.unopK op) :: K⟩
+| While (c : Expr) (body : Stmt) :
+  Eval
+    ⟨.sourceStmt (.While c body), E, K⟩
+    ⟨.sourceExpr c, ∅ :: E, (.loopK c body) :: (.jumpK E.length) :: K⟩
+/-| Break  :
+  Eval
+    ⟨.sourceStmt (.Break), E, K⟩
+    ⟨.skip, E.drop 1, popK K (E.length - 1)⟩
+-/
+-- # Cont
+| IfTrue (s₁ s₂ : Stmt) :
+  Eval
+    ⟨.value .True, E, .ifCondK s₁ s₂ :: K⟩
+    ⟨.sourceStmt s₁, ∅ :: E, (.jumpK E.length) :: K⟩
+| IfFalse (s₁ s₂ : Stmt) :
+  Eval
+    ⟨.value .False, E, .ifCondK s₁ s₂ :: K⟩
+    ⟨.sourceStmt s₂, ∅ :: E, (.jumpK E.length) :: K⟩
+| ScopeDone (l : Nat) :
+  Eval
+    ⟨.skip, E, .jumpK l :: K⟩
+    ⟨.skip, E.drop (E.length - l), K⟩
+| VarDeclDone (x : VarName) (type : τ) (v : Value) :
+  Eval
+    ⟨.value v, E, .declK x type :: K⟩
+    ⟨.skip, insert_first x v E, K⟩
+| AssignDone (x : VarName) (v : Value) :
+  Eval
+    ⟨.value v, E, .assignK x :: K⟩
+    ⟨.skip, modify_first x v E, K⟩
+| SeqDone (s₂ : Stmt) :
+  Eval
+    ⟨.skip, E, .seqK s₂ :: K⟩
+    ⟨.sourceStmt s₂, E, K⟩
+| BinOpL (op : BinOp) (v₁ : Value) (e₂ : Expr) :
+  Eval
+    ⟨.value v₁, E, .binopLK op e₂ :: K⟩
+    ⟨.sourceExpr e₂, E, .binopRK op v₁ :: K⟩
+| BinOpR (op : BinOp) (v₁ : Value) (v₂ : Value) :
+  Eval
+    ⟨.value v₂, E, .binopRK op v₁ :: K⟩
+    ⟨.value (op.run v₁ v₂), E, K⟩
+| LoopTrue (body : Stmt) (c : Expr) :
+  Eval
+    ⟨.value .True, E, .loopK c body :: K⟩
+    ⟨.sourceStmt body, E, .loopK c body :: K⟩
+| LoopFalse (body : Stmt) (c : Expr) :
+  Eval
+    ⟨.value .False, E, .loopK c body :: K⟩
+    ⟨.skip, E, K⟩
+| LoopCont (body : Stmt) (c : Expr) :
+  Eval
+    ⟨.skip, E, .loopK c body :: K⟩
+    ⟨.sourceExpr c, ∅ :: E.drop 1, .loopK c body :: K⟩
+
+def init_state (s : Stmt) : CEK := ⟨.sourceStmt s, [], []⟩
+
+def terminal_state (E : Environment) : CEK := ⟨.skip, E, []⟩
